updated Nomimal-CompCert and Stack-Aware-Nominal-Compert

Nominal-CompCert/common/Memory.v
@@ -155,22 +155,20 @@ Proof.
   auto.
 Qed.
 
-Definition sup_add(b:block)(s:sup) := b::s.
-
-Definition sup_incr(s:sup) := sup_add (fresh_block s) s.
+Definition sup_incr(s:sup) := (fresh_block s) :: s.
 
 Definition sup_include(s1 s2:sup) := forall b, sup_In b s1 -> sup_In b s2.
 
-Theorem sup_add_in : forall b s b', sup_In b' (sup_add b s) <-> b' = b \/ sup_In b' s.
+Theorem sup_incr_in : forall b s, sup_In b (sup_incr s) <-> b = (fresh_block s) \/ sup_In b s.
 Proof.
-  split.
-  intros. destruct H. left. auto. right. auto.
-  intros. destruct H. left. auto. right. auto.
+  split; intro; inv H; simpl in *; auto.
 Qed.
-Theorem sup_add_in1 : forall b s, sup_In b (sup_add b s).
-Proof. intros. apply sup_add_in. left. auto. Qed.
-Theorem sup_add_in2 : forall b s, sup_include s (sup_add b s).
-Proof. intros. intro. intro. apply sup_add_in. right. auto. Qed.
+
+Theorem sup_incr_in1 : forall s, sup_In (fresh_block s) (sup_incr s).
+Proof. intros. apply sup_incr_in. left. auto. Qed.
+Theorem sup_incr_in2 : forall s, sup_include s (sup_incr s).
+Proof. intros. intro. intro. apply sup_incr_in. right. auto. Qed.
+
 
 Lemma sup_include_refl : forall s:sup, sup_include s s.
 Proof. intro. intro. auto. Qed.
@@ -182,9 +180,9 @@ Proof.
 Qed.
 
 Lemma sup_include_incr:
-  forall s b, sup_include s (sup_add b s).
+  forall s, sup_include s (sup_incr s).
 Proof.
-  intros. apply sup_add_in2.
+  intros. apply sup_incr_in2.
 Qed.
 
 End Sup.
@@ -501,12 +499,12 @@ Program Definition empty: mem :=
   infinite memory. *)
 Lemma mem_incr_1: forall m, sup_In (nextblock m) (sup_incr (m.(support))).
 Proof.
-  intros. unfold nextblock. unfold sup_incr. apply sup_add_in1.
+  intros. unfold nextblock. unfold sup_incr. apply sup_incr_in1.
 Qed.
 
 Lemma mem_incr_2: forall m b, sup_In b (m.(support)) -> sup_In b (sup_incr (m.(support))).
 Proof.
-  intros. unfold sup_incr. apply sup_add_in2. auto.
+  intros. unfold sup_incr. apply sup_incr_in2. auto.
 Qed.
 
 Program Definition alloc (m: mem) (lo hi: Z) :=
@@ -1908,7 +1906,7 @@ Theorem valid_block_alloc_inv:
 Proof.
   unfold valid_block; intros.
   rewrite support_alloc in H. rewrite alloc_result.
-  apply sup_add_in. auto.
+  apply sup_incr_in. auto.
 Qed.
 
 Theorem perm_alloc_1:
@@ -4455,7 +4453,7 @@ Theorem alloc_inject_neutral:
   forall s m lo hi b m',
   alloc m lo hi = (m', b) ->
   inject_neutral s m ->
-  sup_include (sup_add b (support m)) s ->
+  sup_include (sup_incr (support m)) s ->
   inject_neutral s m'.
 Proof.
   intros; red.
@@ -4466,7 +4464,8 @@ Proof.
   apply perm_implies with Freeable; auto with mem.
   eapply perm_alloc_2; eauto. lia.
   unfold flat_inj. apply pred_dec_true.
-  apply H1. apply sup_add_in1.
+  apply H1. apply alloc_result in H. subst.
+  apply sup_incr_in1.
 Qed.
 
 Theorem store_inject_neutral:
@@ -4656,7 +4655,7 @@ Lemma alloc_unchanged_on:
   unchanged_on m m'.
 Proof.
   intros; constructor; intros.
-- rewrite (support_alloc _ _ _ _ _ H). intro. intro. apply sup_add_in2. auto.
+- rewrite (support_alloc _ _ _ _ _ H). intro. intro. apply sup_incr_in2. auto.
 - split; intros.
   eapply perm_alloc_1; eauto.
   eapply perm_alloc_4; eauto.
@@ -4720,13 +4719,12 @@ Notation mem := Mem.mem.
 Notation sup := Mem.sup.
 Notation sup_In := Mem.sup_In.
 Notation sup_incr := Mem.sup_incr.
-Notation sup_add := Mem.sup_add.
 Notation sup_empty := Mem.sup_empty.
 Notation fresh_block := Mem.fresh_block.
 Notation freshness := Mem.freshness.
 Global Opaque Mem.alloc Mem.free Mem.store Mem.load Mem.storebytes Mem.loadbytes.
 
-Hint Resolve Mem.sup_add_in1 Mem.sup_add_in2 : core.
+Hint Resolve Mem.sup_incr_in1 Mem.sup_incr_in2 : core.
 Hint Resolve
   Mem.valid_not_valid_diff
   Mem.perm_implies
