Stack-Aware-Nominal-CompCert/driver/Compiler.v
@@ -28,8 +28,6 @@ Require LTL.
 Require Linear.
 Require Mach.
 Require Asm.
-Require SSAsm.
-Require RealAsm.
 (** Translation passes. *)
 Require Initializers.
 Require SimplExpr.
@@ -52,7 +50,6 @@ Require CleanupLabels.
 Require Debugvar.
 Require Stacking.
 Require Asmgen.
-Require RealAsmgen.
 
 (** Proofs of semantic preservation. *)
 Require SimplExprproof.
@@ -76,8 +73,6 @@ Require CleanupLabelsproof.
 Require Debugvarproof.
 Require Stackingproof.
 Require Asmgenproof.
-Require SSAsmproof.
-Require RealAsmproof.
 (** Command-line flags. *)
 Require Import Compopts.
 
@@ -153,8 +148,7 @@ Definition transf_rtl_program (f: RTL.program) : res Asm.program :=
   @@@ partial_if Compopts.debug (time "Debugging info for local variables" Debugvar.transf_program)
   @@@ time "Mach generation" Stacking.transf_program
    @@ print print_Mach
-  @@@ time "Asm generation" Asmgen.transf_program
-   @@ time "SSAsm" SSAsmproof.transf_program.
+  @@@ time "Asm generation" Asmgen.transf_program.
 
 Definition transf_cminor_program (p: Cminor.program) : res Asm.program :=
    OK p
@@ -176,10 +170,11 @@ Definition transf_c_program (p: Csyntax.program) : res Asm.program :=
   @@@ time "Clight generation" SimplExpr.transl_program
   @@@ transf_clight_program.
 
-Definition transf_c_program_real p: res Asm.program :=
+(* Definition transf_c_program_real p: res Asm.program :=
   transf_c_program p
+  @@ time "SSAsm" SSAsmproof.transf_program.
   @@@ time "Translation from SSAsm to RealAsm" RealAsmgen.transf_program.
-
+*)
 (** Force [Initializers] and [Cexec] to be extracted as well. *)
 
 Definition transl_init := Initializers.transl_init.
@@ -265,12 +260,12 @@ Definition CompCert's_passes :=
   ::: mkpass (match_if Compopts.debug Debugvarproof.match_prog)
   ::: mkpass Stackingproof.match_prog
   ::: mkpass Asmgenproof.match_prog
-  ::: mkpass SSAsmproof.match_prog
   ::: pass_nil _.
 
-Definition real_asm_passes :=
-      mkpass RealAsmproof.match_prog
-  ::: pass_nil _.
+(* Definition real_asm_passes :=
+      mkpass SSAsmproof.match_prog
+  ::: mkpass RealAsmproof.match_prog
+  ::: pass_nil _. *)
 (** Composing the [match_prog] relations above, we obtain the relation
   between CompCert C sources and Asm code that characterize CompCert's
   compilation. *)
@@ -284,8 +279,9 @@ Fixpoint passes_app {A B C} (l1: Passes A B) (l2: Passes B C) : Passes A C :=
   | pass_cons _ _ _ P1 l1 => fun l2 => P1 ::: passes_app l1 l2
   end l2.
 
-Definition match_prog_real :=
-  pass_match (compose_passes (passes_app CompCert's_passes real_asm_passes)).
+(* Definition match_prog_real :=
+  pass_match (compose_passes (passes_app CompCert's_passes real_asm_passes)). *)
+
 (** The [transf_c_program] function, when successful, produces
   assembly code that is in the [match_prog] relation with the source C program. *)
 
@@ -343,8 +339,8 @@ Proof.
   exists p18; split. apply CleanupLabelsproof.transf_program_match; auto.
   exists p19; split. eapply partial_if_match; eauto. apply Debugvarproof.transf_program_match.
   exists p20; split. apply Stackingproof.transf_program_match; auto.
-  exists p21; split. apply Asmgenproof.transf_program_match; auto.
-  exists p21; split. eapply SSAsmproof.transf_program_match; auto.
+  exists tp; split. apply Asmgenproof.transf_program_match; auto.
+(*  exists p21; split. eapply SSAsmproof.transf_program_match; auto. *)
   reflexivity.
 Qed.
 
@@ -357,7 +353,7 @@ Proof.
   intros (pi & EQ & CP); inv EQ; auto.
   setoid_rewrite IHA. split; intro H; decompose [ex and] H; eauto.
 Qed.
-
+(*
 Theorem transf_c_program_real_match:
   forall p tp,
     transf_c_program_real p = OK tp ->
@@ -374,7 +370,7 @@ Proof.
   simpl. eexists; split; eauto.
   eapply RealAsmproof.transf_program_match; eauto.
 Qed.
-
+*)
 
 (** * Semantic preservation *)
 
@@ -463,8 +459,8 @@ Qed.
 Theorem cstrategy_semantic_preservation:
   forall p tp,
   match_prog p tp ->
-  forward_simulation (Cstrategy.semantics (fn_stack_requirements tp) p) (SSAsm.semantics tp)
-  /\ backward_simulation (atomic (Cstrategy.semantics (fn_stack_requirements tp) p)) (SSAsm.semantics tp).
+  forward_simulation (Cstrategy.semantics (fn_stack_requirements tp) p) (Asm.semantics tp)
+  /\ backward_simulation (atomic (Cstrategy.semantics (fn_stack_requirements tp) p)) (Asm.semantics tp).
 Proof.
   intros p tp M. unfold match_prog, pass_match in M; simpl in M.
 Ltac DestructM :=
@@ -474,7 +470,7 @@ Ltac DestructM :=
       destruct H as (p & M & MM); clear H
   end.
   repeat DestructM. subst tp.
-  assert (F: forward_simulation (Cstrategy.semantics (fn_stack_requirements p22) p) (SSAsm.semantics p22)).
+  assert (F: forward_simulation (Cstrategy.semantics (fn_stack_requirements p22) p) (Asm.semantics p22)).
   {
   eapply compose_forward_simulations.
     eapply SimplExprproof.transl_program_correct; eassumption.
@@ -520,28 +516,26 @@ Ltac DestructM :=
     exact Asmgenproof.return_address_exists.
     eassumption.
     eapply Asmgen_fn_stack_requirements_match; eauto.
-  eapply compose_forward_simulations.
   eapply Asmgenproof.transf_program_correct; eassumption.
-  eapply SSAsmproof.transf_program_correct.
+(*  eapply SSAsmproof.transf_program_correct.
   eapply Asmgenproof.transf_program_unchange_rsp; eauto.
-  eapply match_program_no_more_functions; eauto. }
-  split. inv M21. auto.
+  eapply match_program_no_more_functions; eauto. *) }
+  split. auto.
   apply forward_to_backward_simulation.
-  inv M21.
   apply factor_forward_simulation. auto. eapply sd_traces.
-  eapply SSAsm.semantics_determinate.
+  eapply Asm.semantics_determinate.
   apply atomic_receptive. apply Cstrategy.semantics_strongly_receptive.
-  apply SSAsm.semantics_determinate.
+  apply Asm.semantics_determinate.
 Qed.
 
 Theorem c_semantic_preservation:
   forall p tp,
   match_prog p tp ->
-  backward_simulation (Csem.semantics (fn_stack_requirements tp) p) (SSAsm.semantics tp).
+  backward_simulation (Csem.semantics (fn_stack_requirements tp) p) (Asm.semantics tp).
 Proof.
   intros.
   apply compose_backward_simulation with (atomic (Cstrategy.semantics (fn_stack_requirements tp) p)).
-  eapply sd_traces; eapply SSAsm.semantics_determinate.
+  eapply sd_traces; eapply Asm.semantics_determinate.
   apply factor_backward_simulation.
   apply Cstrategy.strategy_simulation.
   apply Csem.semantics_single_events.
@@ -549,6 +543,7 @@ Proof.
   exact (proj2 (cstrategy_semantic_preservation _ _ H)).
 Qed.
 
+(*
 Lemma match_prog_wf:
   forall p tp,
     match_prog p tp ->
@@ -584,6 +579,7 @@ Proof.
   red. intros. exploit AsmFacts.in_find_instr; eauto.
   intros [ofs H2]. eapply A; eauto.
 Qed.
+*)
 (** * Correctness of the CompCert compiler *)
 
 (** Combining the results above, we obtain semantic preservation for two
@@ -599,11 +595,11 @@ Qed.
 Theorem transf_c_program_correct:
   forall p tp,
   transf_c_program p = OK tp ->
-  backward_simulation (Csem.semantics (fn_stack_requirements tp) p) (SSAsm.semantics tp).
+  backward_simulation (Csem.semantics (fn_stack_requirements tp) p) (Asm.semantics tp).
 Proof.
   intros. apply c_semantic_preservation. apply transf_c_program_match; auto.
 Qed.
-
+(*
 Theorem transf_c_program_correct_real:
   forall p tp,
   transf_c_program_real p = OK tp ->
@@ -611,7 +607,7 @@ Theorem transf_c_program_correct_real:
 Proof.
   intros. apply c_semantic_preservation_real. apply transf_c_program_real_match; auto.
 Qed.
-
+*)
 (** Here is the separate compilation case.  Consider a nonempty list [c_units]
   of C source files (compilation units), [C1 ,,, Cn].  Assume that every
   C compilation unit [Ci] is successfully compiled by CompCert, obtaining
@@ -630,7 +626,7 @@ Theorem separate_transf_c_program_correct:
   link_list c_units = Some c_program ->
   exists asm_program,
       link_list asm_units = Some asm_program
-   /\ backward_simulation (Csem.semantics (fn_stack_requirements asm_program) c_program) (SSAsm.semantics asm_program).
+   /\ backward_simulation (Csem.semantics (fn_stack_requirements asm_program) c_program) (Asm.semantics asm_program).
 Proof.
   intros.
   assert (nlist_forall2 match_prog c_units asm_units).
@@ -640,7 +636,7 @@ Proof.
   destruct H2 as (asm_program & P & Q).
   exists asm_program; split; auto. apply c_semantic_preservation; auto.
 Qed.
-
+(*
 Theorem separate_transf_c_program_correct_real:
   forall c_units asm_units c_program,
   nlist_forall2 (fun cu tcu => transf_c_program_real cu = OK tcu) c_units asm_units ->
@@ -657,3 +653,4 @@ Proof.
   destruct H2 as (asm_program & P & Q).
   exists asm_program; split; auto. apply c_semantic_preservation_real; auto.
 Qed.
+*)
