Stack-Aware-Nominal-CompCert/driver/Complements.v
@@ -31,7 +31,7 @@ Require Import Compiler.
 Theorem transf_c_program_preservation:
   forall p tp beh,
   transf_c_program p = OK tp ->
-  program_behaves (SSAsm.semantics tp) beh ->
+  program_behaves (Asm.semantics tp) beh ->
   exists beh', program_behaves (Csem.semantics (fn_stack_requirements tp) p) beh' /\ behavior_improves beh' beh.
 Proof.
   intros. eapply backward_simulation_behavior_improves; eauto.
@@ -46,7 +46,7 @@ Theorem transf_c_program_is_refinement:
   forall p tp,
   transf_c_program p = OK tp ->
   (forall beh, program_behaves (Csem.semantics (fn_stack_requirements tp) p) beh -> not_wrong beh) ->
-  (forall beh, program_behaves (SSAsm.semantics tp) beh -> program_behaves (Csem.semantics (fn_stack_requirements tp)p) beh).
+  (forall beh, program_behaves (Asm.semantics tp) beh -> program_behaves (Csem.semantics (fn_stack_requirements tp)p) beh).
 Proof.
   intros. eapply backward_simulation_same_safe_behavior; eauto.
   apply transf_c_program_correct; auto.
@@ -59,14 +59,14 @@ Theorem transf_cstrategy_program_preservation:
   forall p tp,
   transf_c_program p = OK tp ->
   (forall beh, program_behaves (Cstrategy.semantics(fn_stack_requirements tp) p) beh ->
-     exists beh', program_behaves (SSAsm.semantics tp) beh' /\ behavior_improves beh beh')
-/\(forall beh, program_behaves (SSAsm.semantics tp) beh ->
+     exists beh', program_behaves (Asm.semantics tp) beh' /\ behavior_improves beh beh')
+/\(forall beh, program_behaves (Asm.semantics tp) beh ->
      exists beh', program_behaves (Cstrategy.semantics (fn_stack_requirements tp)p) beh' /\ behavior_improves beh' beh)
 /\(forall beh, not_wrong beh ->
-     program_behaves (Cstrategy.semantics (fn_stack_requirements tp)p) beh -> program_behaves (SSAsm.semantics tp) beh)
+     program_behaves (Cstrategy.semantics (fn_stack_requirements tp)p) beh -> program_behaves (Asm.semantics tp) beh)
 /\(forall beh,
      (forall beh', program_behaves (Cstrategy.semantics (fn_stack_requirements tp)p) beh' -> not_wrong beh') ->
-     program_behaves (SSAsm.semantics tp) beh ->
+     program_behaves (Asm.semantics tp) beh ->
      program_behaves (Cstrategy.semantics (fn_stack_requirements tp)p) beh).
 Proof.
   assert (WBT: forall p fsr, well_behaved_traces (Cstrategy.semantics fsr p)).
@@ -96,11 +96,11 @@ Theorem bigstep_cstrategy_preservation:
   transf_c_program p = OK tp ->
   (forall t r,
      Cstrategy.bigstep_program_terminates (fn_stack_requirements tp) p t r ->
-     program_behaves (SSAsm.semantics tp) (Terminates t r))
+     program_behaves (Asm.semantics tp) (Terminates t r))
 /\(forall T,
      Cstrategy.bigstep_program_diverges (fn_stack_requirements tp) p T ->
-       program_behaves (SSAsm.semantics tp) (Reacts T)
-    \/ exists t, program_behaves (SSAsm.semantics tp) (Diverges t) /\ traceinf_prefix t T).
+       program_behaves (Asm.semantics tp) (Reacts T)
+    \/ exists t, program_behaves (Asm.semantics tp) (Diverges t) /\ traceinf_prefix t T).
 Proof.
   intuition.
   apply transf_cstrategy_program_preservation with p; auto. red; auto.
@@ -135,7 +135,7 @@ Definition specification := program_behavior -> Prop.
 Definition c_program_satisfies_spec (p: Csyntax.program) (spec: specification): Prop :=
   forall beh fsr,  program_behaves (Csem.semantics fsr p) beh -> spec beh.
 Definition ssasm_program_satisfies_spec (p: Asm.program) (spec: specification): Prop :=
-  forall beh,  program_behaves (SSAsm.semantics p) beh -> spec beh.
+  forall beh,  program_behaves (Asm.semantics p) beh -> spec beh.
 
 (** It is not always the case that if the source program satisfies a
   specification, then the generated assembly code satisfies it as
@@ -183,7 +183,7 @@ Qed.
 Definition c_program_has_initial_trace (p: Csyntax.program) (t: trace): Prop :=
   forall beh fsr, program_behaves (Csem.semantics fsr p) beh -> behavior_prefix t beh.
 Definition ssasm_program_has_initial_trace (p: Asm.program) (t: trace): Prop :=
-  forall beh, program_behaves (SSAsm.semantics p) beh -> behavior_prefix t beh.
+  forall beh, program_behaves (Asm.semantics p) beh -> behavior_prefix t beh.
 
 Theorem transf_c_program_preserves_initial_trace:
   forall p tp t,
@@ -243,7 +243,7 @@ Let compiled_linking: link_list asm_units = Some asm_program := proj2_sig compil
 
 Theorem separate_transf_c_program_preservation:
   forall beh,
-  program_behaves (SSAsm.semantics asm_program) beh ->
+  program_behaves (Asm.semantics asm_program) beh ->
   exists beh', program_behaves (Csem.semantics (fn_stack_requirements asm_program) c_program) beh' /\ behavior_improves beh' beh.
 Proof.
   intros. exploit separate_transf_c_program_correct; eauto. intros (a & P & Q).
@@ -256,7 +256,7 @@ Qed.
 
 Theorem separate_transf_c_program_is_refinement:
   (forall beh, program_behaves (Csem.semantics (fn_stack_requirements asm_program) c_program) beh -> not_wrong beh) ->
-  (forall beh, program_behaves (SSAsm.semantics asm_program) beh -> program_behaves (Csem.semantics (fn_stack_requirements asm_program)c_program) beh).
+  (forall beh, program_behaves (Asm.semantics asm_program) beh -> program_behaves (Csem.semantics (fn_stack_requirements asm_program)c_program) beh).
 Proof.
   intros. exploit separate_transf_c_program_preservation; eauto. intros (beh' & P & Q).
   assert (not_wrong beh') by auto.
